Start type safety stuff

theories/Test.v
@@ -3,9 +3,6 @@ Require Import Relations.Relation_Operators.
 Require Import Program.Equality List Lia.
 Require Import Autosubst.Autosubst.
 
-Print rename.
-Print subst.
-
 Inductive type : Type :=
 | Bool
 | Arr (t1 t2 : type).
@@ -31,6 +28,12 @@ Inductive value : term → Prop :=
 
 #[export] Hint Constructors value : core.
 
+Lemma value_dec : forall v, value v ∨ ¬ (value v).
+Proof.
+  destruct v; auto; right; intros H; inversion H.
+Qed.
+
+
 Reserved Notation "e '-->' e'" (at level 80).
 Inductive step : term -> term -> Prop :=
 | step_beta : ∀ T e v u, value v → u = e.[v .: ids] → TApp (TLam T e) v --> u
@@ -48,6 +51,27 @@ Definition multistep := clos_refl_trans_1n _ step.
 Notation "e '-->*' e'" := (multistep e e') (at level 80).
 #[export] Hint Constructors clos_refl_trans_1n : core.
 
+Definition nf (t : term) := ∀ t', ¬ (t --> t').
+Lemma value_is_nf : ∀ v, value v → nf v.
+Proof.
+  intros v Hv.
+  destruct Hv; intros t' Hstep; inversion Hstep.
+Qed.
+Ltac value_step :=
+  match goal with
+  | [ Hv : TLam ?T ?e --> _ |- _ ] => inversion Hv
+  | [ Hv : TTrue --> _ |- _ ] => inversion Hv
+  | [ Hv : TFalse --> _ |- _ ] => inversion Hv
+  | [ Hv : value ?v, Hstep : ?v --> ?e  |- _ ] => exfalso; apply (value_is_nf _ Hv _ Hstep)
+  end.
+
+Lemma value_multistep : ∀ v v', value v → v -->* v' → v' = v.
+Proof.
+  intros.
+  inversion H0. auto.
+  value_step.
+Qed.
+
 Section Examples.
   Definition e_id := TLam Bool (TVar 0).
   Goal TApp e_id TTrue --> TTrue.
@@ -58,21 +82,6 @@ Section Examples.
 End Examples.
 
 Section Deterministic.
-  Definition nf (t : term) := ∀ t', ¬ (t --> t').
-  Lemma value_is_nf : ∀ v, value v → nf v.
-  Proof.
-    intros v Hv.
-    destruct Hv; intros t' Hstep; inversion Hstep.
-  Qed.
-
-  Ltac value_step :=
-    match goal with
-    | [ Hv : TLam ?T ?e --> _ |- _ ] => inversion Hv
-    | [ Hv : TTrue --> _ |- _ ] => inversion Hv
-    | [ Hv : TFalse --> _ |- _ ] => inversion Hv
-    | [ Hv : value ?v, Hstep : ?v --> ?e  |- _ ] => exfalso; apply (value_is_nf _ Hv _ Hstep)
-    end.
-
   Theorem step_deterministic : ∀ {s t₁ t₂ : term},
       s --> t₁ →
       s --> t₂ →
@@ -109,7 +118,7 @@ Section Deterministic.
 End Deterministic.
 
 
-
+(*
 Definition context := var → option type.
 Definition empty : context := fun _ => None.
 
@@ -120,21 +129,195 @@ Proof.
   exact (Γ (ρ x)).
 Defined.
 
-Print Rename.
-Print Subst.
 Definition shift_ctx : type → context → context :=
   fun T Γ x => match x with
                | O => Some T
                | S n => Γ n
                end.
+*)
+
+Definition context := list type.
+Definition empty : context := nil.
+
+Definition lookup : context → nat → option type := @nth_error type.
 
 Reserved Notation "Γ '⊢' e '∈' T'" (at level 85).
 Inductive has_type : context → term → type → Prop :=
+| type_var : ∀ Γ x τ, lookup Γ x = Some τ → Γ ⊢ TVar x ∈ τ
 | type_true : ∀ Γ, Γ ⊢ TTrue ∈ Bool
 | type_false : ∀ Γ, Γ ⊢ TFalse ∈ Bool
-| type_lam : ∀ Γ e τ₁ τ₂, (shift_ctx τ₁ Γ) ⊢ e ∈ τ₂ → Γ ⊢ TLam τ₁ e ∈ τ₁ ⇒ τ₂
+| type_lam : ∀ Γ e τ₁ τ₂, (τ₁ :: Γ) ⊢ e ∈ τ₂ → Γ ⊢ TLam τ₁ e ∈ τ₁ ⇒ τ₂
 | type_app : ∀ Γ f e τ τ₂, Γ ⊢ f ∈ τ₂ ⇒ τ → Γ ⊢ e ∈ τ₂ → Γ ⊢ TApp f e ∈ τ
 | type_if : ∀ Γ e e₁ e₂ τ, Γ ⊢ e ∈ Bool → Γ ⊢ e₁ ∈ τ → Γ ⊢ e₂ ∈ τ → Γ ⊢ TIf e e₁ e₂ ∈ τ
 where "Γ '⊢' e '∈' T" := (has_type Γ e T).
+Notation "'⊢' e '∈' T" := (empty ⊢ e ∈ T) (at level 85).
 
-Check subst_comp.
+
+Section TypeSafety.
+  Definition safe (e : term) := forall e', e -->* e' → value e' ∨ ∃ e'', e' --> e''.
+
+  (*
+  This definition doesn't work: runs into positivity requirement.
+  Inductive sem_value : type → term → Prop :=
+  | sem_value_true : sem_value Bool TTrue
+  | sem_value_false : sem_value Bool TFalse
+  | sem_value_arr : ∀ τ₁ τ₂ e, (∀ v, value v → sem_value τ₁ v → sem_expr τ₂ e.[v/]) → sem_value (τ₁ ⇒ τ₂) (TLam τ₁ e)
+  with sem_expr : type → term → Prop :=
+  | sem_exprC : ∀ τ e, (∀ e', e -->* e' → (* irred(e') → *) sem_value τ e') → sem_expr τ e.
+  *)
+
+  Definition irred (e : term) := forall e', ¬ (e --> e').
+  Ltac irred_step :=
+    match goal with
+    | [ H : irred ?e, Hstep : ?e --> ?e' |- _ ] => exfalso; apply H in Hstep; assumption
+    end.
+
+  Axiom LEM : ∀ P, P ∨ ¬ P.
+  Lemma irred_decidable : ∀ e, (∃ e', e --> e') ∨ irred e.
+  Proof.
+    intros e.
+    destruct (LEM (∃ e', e --> e')); auto.
+    right.
+    intros e' Hstep.
+    eauto.
+  Qed.
+
+  (*
+    induction e.
+    - right. intros e' H. value_step.
+    - right. intros e' H. value_step.
+    - destruct e1; try solve [left; eexists; auto];
+        repeat (destruct IHe1 as [[e1' ?] | ?]; [
+        left; eexists; apply step_if; apply H |
+        right; intros e' Hstep; inversion Hstep; subst; irred_step ]).
+    - right. intros e' H. inversion H.
+    - right. intros e' H. value_step.
+    - destruct IHe1 as [[e1' ?] | ?].
+      left. eexists. constructor. apply H.
+      destruct IHe2 as [[e2' ?] | ?].
+      destruct (value_dec e1).
+      * left. eexists. apply step_app2. apply H1. apply H0.
+      * right. intros e' Hstep. inversion Hstep; subst. value_step. irred_step. apply H1. assumption.
+
+      * destruct (value_dec e1).
+        destruct (value_dec e2).
+  Admitted. *)
+
+
+  (* The easiest way to write this is to avoid mutual recursion altogether, since Coq's termination checker isn't smart enough to see that this is well-founded. *)
+  Fixpoint sem_value (T : type) : term → Prop :=
+    match T with
+    | Bool => fun t => t = TTrue ∨ t = TFalse
+    | τ₁ ⇒ τ₂ => fun t => ∃ e, t = TLam τ₁ e ∧ (∀ v, sem_value τ₁ v →
+              (∀ e', e.[v/] -->* e' → irred e' → sem_value τ₂ e'))
+                                                end.
+  Definition sem_expr (τ : type) : term → Prop :=
+        fun e => ∀ e', e -->* e' → irred e' → sem_value τ e'.
+
+  Notation "v '∈' '𝓥⟦' τ '⟧'" := (sem_value τ v) (at level 80).
+  Notation "e '∈' '𝓔⟦' τ '⟧'" := (sem_expr τ e) (at level 80).
+
+  Lemma sem_val_is_sem_expr : forall v τ, v ∈ 𝓥⟦ τ ⟧ → v ∈ 𝓔⟦ τ ⟧.
+  Proof.
+    intros v τ H.
+    destruct τ.
+    - destruct H; intros e' Hstep; subst; apply value_multistep in Hstep; subst; simpl; auto.
+    - simpl in H.
+      destruct H as [e [H1 H2]].
+      subst.
+      intros e' Hstep. apply value_multistep in Hstep; subst; simpl; auto.
+      intros.
+      eexists. split. reflexivity.
+      apply H2.
+  Qed.
+
+  Definition id_subst : var → term := ids.
+  Inductive valid_subst : context → (var → term) → Prop :=
+  | subst_empty : valid_subst empty id_subst
+  | subst_cons : ∀ Γ γ v τ, valid_subst Γ γ → v ∈ 𝓥⟦ τ ⟧ → valid_subst (τ :: Γ) (v .: γ).
+  #[local] Hint Constructors valid_subst : core.
+
+  Lemma valid_subst_var : ∀ Γ γ, valid_subst Γ γ → ∀ x τ, lookup Γ x = Some τ → γ x ∈ 𝓥⟦ τ ⟧.
+  Proof.
+    intros Γ γ H.
+    induction H; intros.
+    - destruct x; simpl in *; discriminate.
+    - induction x. simpl in *. inversion H1. subst. assumption.
+      simpl in *. apply IHvalid_subst. assumption.
+  Qed.
+
+    (* Lemma: if e has type τ in Γ, and γ is a valid substitution, then e.[γ] is closed term and has type τ in empty context*)
+
+  Definition sem_has_type (Γ : context) (e : term) (τ : type) :=
+    ∀ (γ : var → term), valid_subst Γ γ → e.[γ] ∈ 𝓔⟦ τ ⟧.
+  (* Need that γ is a correct substitution according to Γ, that e.[γ] is closed and so on *)
+  Notation "Γ '⊧' e '∈' τ" := (sem_has_type Γ e τ) (at level 80).
+  Notation "'⊧' e '∈' T" := (empty ⊧ e ∈ T) (at level 85).
+
+  Lemma sem_value_is_value : ∀ v τ, v ∈ 𝓥⟦ τ ⟧ → value v.
+  Proof.
+    intros v τ H.
+    destruct τ.
+    - unfold sem_value in H.
+      destruct H; rewrite H; auto.
+    - destruct H as [H1 [H2 H3]].
+      rewrite H2.
+      auto.
+  Qed.
+
+  Lemma fund_lemma : ∀ e τ, ⊢ e ∈ τ → ⊧ e ∈ τ.
+  Proof.
+    intros e τ He.
+    induction He; intros γ Hγ; simpl.
+    - (* Var case *)
+      apply sem_val_is_sem_expr.
+      eapply valid_subst_var; eauto.
+    - apply sem_val_is_sem_expr; simpl; auto.
+    - apply sem_val_is_sem_expr; simpl; auto.
+    - (* Lambda case *) intros e' Hstep.
+      assert (e' = TLam τ₁ e.[up γ]). { apply value_multistep; auto. }
+      rewrite H.
+      intros.
+      simpl.
+      eexists; split; auto.
+      intros v Hv.
+      unfold sem_has_type in IHHe.
+      specialize IHHe with (v .: γ).
+      rewrite subst_comp. simpl.
+      assert (e.[up γ >> v .: ids] = e.[v .: γ]). { autosubst. }
+      rewrite H1.
+      unfold sem_expr in IHHe.
+      apply IHHe.
+      constructor; auto.
+    - (* App case *) admit.
+    - (* If case *) unfold sem_has_type in IHHe1, IHHe2, IHHe3.
+      specialize IHHe1 with γ.
+      intros e' Hstep He'.
+      unfold sem_expr in IHHe1.
+      admit.
+  Admitted.
+
+  (* Need a bunch of congruence step lemmas: *)
+
+
+
+  Lemma sem_type_implies_safe : ∀ e τ, ⊧ e ∈ τ → safe e.
+  Proof.
+    intros e τ H.
+    unfold sem_has_type in H.
+    specialize H with id_subst.
+    unfold id_subst in H.
+    rewrite subst_id in H.
+    intros e' He'.
+    destruct (irred_decidable e').
+    - right. assumption.
+    - left.
+      eapply sem_value_is_value. apply H; eauto.
+  Qed.
+
+  Theorem type_safety : ∀ τ t, ⊢ t ∈ τ → safe t.
+  Proof.
+    eauto using fund_lemma, sem_type_implies_safe.
+  Qed.
+
+End TypeSafety.
